examples/IOCO_ex.v
@@ -80,7 +80,7 @@ Proof.
   unfold ind_out in H3. destruct H3 as [H3 _].
   unfold ind_out in H4. destruct H4 as [_ H4].
   apply H3 in H5. destruct H5 as [s' [so' [H5_1 [H5_2 H5_3]]]].
-  unfold ind_s_after_IOLTS in H1. simpl in H1. unfold ind_s_after in H1.
+  unfold ind_s_after_IOLTS in H1. vm_compute q0 in H1. unfold ind_s_after in H1.
   apply H1 in H5_1.
   unfold ind_s_after_IOLTS in H2. simpl in H2. unfold ind_s_after in H2.
   remember H as H'. clear HeqH'. apply H2 in H'. apply H4 in H'.
@@ -95,91 +95,107 @@ Proof.
     clear IHt'. destruct t' as [| a t'']; [| destruct a].
     + (* t = [ s_event "a" ] *)
       expand_s_seq_reachability H.
-      expand_s_seq_reachability H5_1. expand_out_one_state H5_2 x H5_3.
-      clear H_so H5_1 H5_2 H0 H1 H4. inversion H'; [expand_In H0 |].
-      apply H2. exists 3. split; try apply transition_r1; elem_in_list.
+      expand_s_seq_reachability H5_1; expand_out_one_state H5_2 x H5_3;
+      clear H_so H5_1 H5_2 H0 H1; inversion H'; try (expand_In H0);
+      apply H3; exists 2; split; try apply transition_r1; elem_in_list.
     + (* t = s_event "a" :: s_event "x" :: t'' => induction t'' *)
       induction t'' as [| a t''' IHt''']; [| destruct a].
       * (* t = [ s_event "a"; s_event "x" ] *)
         expand_s_seq_reachability H.
-        expand_s_seq_reachability H5_1; expand_out_one_state H5_2 x H5_3.
-        clear H0 H1 H2 H3 H4. inversion H'; [elem_in_list |].
-        destruct H0. elem_in_list.
+        expand_s_seq_reachability H5_1; expand_out_one_state H5_2 x H5_3;
+        clear H0 H1 H2 H3 H4; inversion H'; try (elem_in_list);
+        destruct H0; elem_in_list.
       * (* t = s_event _ :: s_event _ :: s_event _ :: t'' => contradiction *)
         expand_s_seq_reachability H.
       * (* t = s_event "a" :: s_event "x" :: delta :: t''' => use IHt''' *)
         apply IHt'''.
         -- inversion H. subst. expand_one_step_reachability H3.
-           apply s_seq_reachability_r2 with (si := 2); auto.
+           apply s_seq_reachability_r2 with (si := 0); auto.
            inversion H6. subst. expand_one_step_reachability H5.
-           apply s_seq_reachability_r2 with (si := 3); auto.
+           apply s_seq_reachability_r2 with (si := 2); auto.
            inversion H9. subst. apply H8.
-        -- inversion H5_1. subst. expand_one_step_reachability H3;
-           eapply s_seq_reachability_r2; try (apply H3);
-           inversion H6; subst; expand_one_step_reachability H5;
-           eapply s_seq_reachability_r2; try (apply H5); inversion H9; auto.
+        -- inversion H5_1 as [| ? ? ? ? ? ? H_one_step H_seq |]. subst.
+           expand_one_step_reachability H_one_step;
+           eapply s_seq_reachability_r2; try (apply H_one_step);
+           inversion H_seq as [| ? ? ? ? ? ? H_one_step2 H_seq2 |]; subst;
+           expand_one_step_reachability H_one_step2;
+           eapply s_seq_reachability_r2;
+           try (apply H_one_step2);
+           inversion H_seq2 as [| | ? ? ? ? ? H_seq3 ]; apply H_seq3.
     + (* t = s_event "a" :: delta :: t'' => contradiction *)
       expand_s_seq_reachability H.
   - (* t = delta :: t' => use IHt' *)
-    inversion H5_1. subst. inversion H. subst. apply IHt'; auto.
+    inversion H5_1. subst. inversion H. subst. apply IHt'.
+    + apply H5.
+    + apply H3.
 Qed.
 
 Example i1_not_ioco_s3 : ~ (ind_ioco imp_i1 spec_s3_IOLTS).
 Proof.
   unfold ind_ioco. unfold not. intros H. simpl in H.
-  specialize (H [1] [4] [s_event "b"] [delta] [s_event "y"] ).
+  specialize (H [0; 1] [2] [s_event "b"] [delta] [s_event "y"] ).
   assert ( H': ~ incl [delta] [s_event "y"]).
   { unfold incl. intros H''. specialize (H'' delta). destruct H'';
     try inversion H0. left. reflexivity.
   }
   apply H'. apply H.
-  - unfold ind_s_traces_LTS. unfold ind_s_traces. exists 4. simpl.
-    apply s_seq_reachability_r2 with (si := 4).
-    + apply one_step_reachability_r1 with (s1 := 1) (s2 := 4);
+  - unfold ind_s_traces_LTS. unfold ind_s_traces. exists 2. simpl.
+    apply s_seq_reachability_r2 with (si := 2).
+    + apply one_step_reachability_r1 with (s1 := 1) (s2 := 2);
       try apply empty_reachability_r1.
       apply transition_r1. elem_in_list.
     + apply s_seq_reachability_r1. apply empty_reachability_r1.
   - unfold ind_s_after_IOLTS. unfold ind_s_after. intros a. split.
-    + simpl. intros H''. inversion H''; subst. simpl in *. inversion H3; subst.
-      inversion H0; subst.
-      * inversion H1; subst. expand_In H7. subst. inversion H2; subst.
-        -- inversion H6; subst. simpl in H4. inversion H4; subst.
-           ++ left. reflexivity.
-           ++ inversion H5; subst. expand_In H9.
-        -- inversion H4; subst. expand_In H8.
-      * inversion H4; subst. expand_In H7.
-    + intros H''. expand_In H''. simpl. apply s_seq_reachability_r2 with (si := 1).
-      * apply one_step_reachability_r1 with (s1 := 1) (s2 := 1);
-        try apply empty_reachability_r1.
-        apply transition_r1. elem_in_list.
-      * apply s_seq_reachability_r1. apply empty_reachability_r1.
+    + simpl. intros H''. vm_compute BE_trans_set_converter.startState in H''.
+      expand_s_seq_reachability H''; elem_in_list.
+    + intros H''. expand_In H''; vm_compute q0.
+      * apply s_seq_reachability_r2 with (si := 0).
+        -- apply one_step_reachability_r1 with (s1 := 1) (s2 := 0);
+           try apply empty_reachability_r1.
+           apply transition_r1. vm_compute T. elem_in_list.
+        -- apply s_seq_reachability_r1. apply empty_reachability_r1.
+      * apply s_seq_reachability_r2 with (si := 0).
+        -- apply one_step_reachability_r1 with (s1 := 1) (s2 := 0);
+           try apply empty_reachability_r1.
+           apply transition_r1. vm_compute T. elem_in_list.
+        -- apply s_seq_reachability_r1. apply empty_reachability_r2 with (si := 1).
+           ++ apply transition_r2. vm_compute T. elem_in_list.
+           ++ apply empty_reachability_r1.
   - unfold ind_s_after_IOLTS. unfold ind_s_after. intros a. split.
     + simpl. intros H''. inversion H''; subst. simpl in *. inversion H3; subst.
       inversion H0; subst.
       * inversion H1; subst. expand_In H7. subst. inversion H2; subst.
         -- inversion H6; subst. simpl in H4. inversion H4; subst.
-           ++ left. reflexivity.
+           ++ left. vm_compute. reflexivity.
            ++ inversion H5; subst. expand_In H9.
         -- inversion H4; subst. expand_In H8.
       * inversion H4; subst. expand_In H7.
-    + intros H''. expand_In H''. simpl. apply s_seq_reachability_r2 with (si := 4).
-      * apply one_step_reachability_r1 with (s1 := 1) (s2 := 4);
+    + intros H''. expand_In H''. simpl. apply s_seq_reachability_r2 with (si := 2).
+      * apply one_step_reachability_r1 with (s1 := 1) (s2 := 2);
         try apply empty_reachability_r1.
         apply transition_r1. elem_in_list.
       * apply s_seq_reachability_r1. apply empty_reachability_r1.
   - unfold ind_out. split.
     + intros l H''. expand_In H''. exists 1. exists [delta].
-      repeat split; try(apply out_one_state_r1); elem_in_list.
-    + intros s H''. expand_In H''. exists [delta]. split.
-      * try(apply out_one_state_r1); elem_in_list.
-      * intros o H'''. expand_In H'''. elem_in_list.
+      repeat split; try (apply out_one_state_r1); vm_compute; elem_in_list.
+    + intros s H''. expand_In H''.
+      * exists []. split; [| intros o H'''; expand_In H'''].
+        apply out_one_state_r2;
+        [ vm_compute Ts; intros H'''; expand_In H''' |
+          intros H'''; expand_In H'''|].
+        intros l. split.
+        -- intros H'''; expand_In H'''.
+        -- intros H'''. destruct H''' as [s' [H'''_1 H'''_2]].
+           expand_transition H'''_2.
+      * exists [delta].  split; [| intros o H'''; expand_In H'''; elem_in_list].
+        apply out_one_state_r1. vm_compute. elem_in_list.
   - unfold ind_out. split.
-    + intros l H''. expand_In H''. exists 4. exists [s_event "y"].
+    + intros l H''. expand_In H''. exists 2. exists [s_event "y"].
       repeat split; try elem_in_list. apply out_one_state_r2.
       * intros H'''; expand_In H'''.
       * intros H'''; expand_In H'''.
       * intros l'. split.
-        -- intros H'''. expand_In H'''. exists 5. split; try (elem_in_list).
+        -- intros H'''. expand_In H'''. exists 3. split; try (elem_in_list).
            apply transition_r1. elem_in_list.
         -- intros H'''. destruct H''' as [ s' [ H'''_1 H'''_2]].
            inversion H'''_2; subst.
@@ -189,7 +205,7 @@ Proof.
         -- intros H'''; expand_In H'''.
         -- intros H'''; expand_In H'''.
         -- intros l'. split.
-           ++ intros H'''. expand_In H'''. exists 5. split; try (elem_in_list).
+           ++ intros H'''. expand_In H'''. exists 3. split; try (elem_in_list).
               apply transition_r1. elem_in_list.
            ++ intros H'''. destruct H''' as [ s' [ H'''_1 H'''_2]].
               inversion H'''_2; subst. expand_In H'''_1; subst; expand_In H3.
